Moved the old evidence and infon types to a more general term type, to more closely match the implementation of the logic engine.

ModularEngine/src/LogicEngine.FStar/coredkal.fst
@@ -36,25 +36,29 @@ type constant =
   | SubstrateConstant : object -> constant 
 
 type relationInfon
-type func
-
-
-
+type func =
+  | EmptyInfon : func
+  | SaidInfon : func
+  | AsInfon : func
+  | AndInfon : func
+  | ImpliesInfon : func
+  | RelationInfon : relationInfon -> func
+  (* ... *)
 
 type substitution
 
+type query (* to be replaced by SubstrateUpdate and SubstrateQuery eventually *)
 
-type term (*= 
+type term = 
   | Var : var -> term
   | Const : constant -> term
   | Forall : var -> term -> term
   | App : func -> list term -> term
+  | SubstrateQueryTerm : query -> term
   (* | ... *)
-*)
-  
-
 
 (** to be replaced **)
+(*
 type query
 
 type evidence =
@@ -74,16 +78,21 @@ type infon =
   | Said : infon -> infon -> infon
 (*                | And i j *)
   | Implies : infon -> infon -> infon
-  
+ *)
   
 (** added here **)
-type infostrate = list infon
+
+type infostrate = list term
 type substrate = list query
 type varDecl = list var
-type prefix = list infon
-(*
-let said (p:term) (i:term) = App(Said, [p; i])
-*)
+type prefix = list term
+
+(* val declarations seem necessary here for funs to be used even in same file *)
+val said : term -> term -> term
+let said (p:term) (i:term) = App SaidInfon [p; i]
+
+val empty : term
+let empty = App EmptyInfon []
   
 (*************)
 (* Utilities *)
@@ -109,26 +118,28 @@ val memSubstrate : q:query -> s:substrate -> option (Mem q s)
 let memSubstrate q _S = mem q _S
   (* Rk: does not accept : let memSubstrate = mem which is essentially the same *)
   
-val memInfostrate : i:infon -> is:infostrate -> option (Mem i is)
+val memInfostrate : i:term -> is:infostrate -> option (Mem i is)
 let memInfostrate i _I = mem i _I
 
 
 (* Intuition:                                                 *)
 (* MkPrefix [p1;...;pn] i (p1 said (p2 said ... (pn said i))) *)
-type MkPrefix :: list infon => infon => infon => P =
-  | MkPrefix_Nil : i:infon -> MkPrefix [] i i
-  | MkPrefix_Cons : p:infon -> ps:list infon -> i:infon -> i':infon 
+type MkPrefix :: list term => term => term => P =
+  | MkPrefix_Nil : i:term -> MkPrefix [] i i
+  | MkPrefix_Cons : p:term -> ps:list term -> i:term -> i':term 
                    -> MkPrefix ps i i'
-                   -> MkPrefix (p::ps) i (Said p i')
+                   -> MkPrefix (p::ps) i (App SaidInfon [p; i'])
+				   (* Rk: cannot use said here *)
 
 (* Intuition:                                                    *) 
 (* mkPrefix [p1;...;pn] i = ( (p1 said (... pn said i)), proof ) *)
-val mkPrefix: pref:prefix -> i:infon -> (i':infon * dummy:(MkPrefix pref i i'){pref=[] => i=i'})
+val mkPrefix: pref:prefix -> i:term -> (i':term * dummy:(MkPrefix pref i i'){pref=[] => i=i'})
 let rec mkPrefix pref i =
   (match pref with
      | [] -> (i, MkPrefix_Nil i)
      | h::t -> let (j, m) = mkPrefix t i in
-	             ((Said h j), MkPrefix_Cons h t i j m))				   
+                 (App SaidInfon [h; j], MkPrefix_Cons h t i j m))
+                 (* Rk: if using the function said here, can't prove it *)				 
 
 
 (***********************)
@@ -137,15 +148,16 @@ let rec mkPrefix pref i =
 
 (*type types :: varDecl => ? => typ => P =*)
 
-type entails :: substrate => infostrate => varDecl => infon => P =
+type entails :: substrate => infostrate => varDecl => term => P =
   | Entails_Emp : S:substrate -> I:infostrate -> G:varDecl
                -> pref: prefix
-			   -> result: infon
-			   -> MkPrefix pref Empty result
+			   -> result: term
+			   -> MkPrefix pref (App EmptyInfon []) result
+			      (* Rk: cannot just use empty in place of App EmptyInfon [] *)
 			   -> entails S I G result
 
   | Entails_Hyp_Knowledge : S:substrate -> I:infostrate -> G:varDecl
-                          -> i:infon
+                          -> i:term
 						  -> Mem i I
 						  -> entails S I G i
 						  
@@ -153,12 +165,13 @@ type entails :: substrate => infostrate => varDecl => infon => P =
                           -> q:query 
                           -> Mem q S  
 						  (* Eventually, we get a signature from the DB about this fact *)
-                          -> entails S I G (AsInfon q)
+                          -> entails S I G (App AsInfon [(SubstrateQueryTerm q)])
+						  (* Rk: need parenthesis inside the list *)
 
   (* Q: here order of G matters; make sure that's all right; I think so *)
   | Entails_Q_Intro : S:substrate -> I:infostrate -> G:varDecl
-                    -> x:var -> i:infon -> i':infon
-					-> result:infon
+                    -> x:var -> i:term -> i':term
+					-> result:term
 					-> pref:prefix
 			        (*-> MkPrefix pref (Forall x i) result *) (* TODO?? *)
 					-> MkPrefix pref i i'
@@ -166,11 +179,11 @@ type entails :: substrate => infostrate => varDecl => infon => P =
 					-> entails S I G result
 				 
   | Entails_And_Intro : S:substrate -> I:infostrate -> G:varDecl
-                     -> i:infon -> i':infon
-                     -> j:infon -> j':infon 
-                     -> result:infon
+                     -> i:term -> i':term
+                     -> j:term -> j':term 
+                     -> result:term
                      -> pref: prefix
-                     -> MkPrefix pref (And i j) result
+                     -> MkPrefix pref (App AndInfon [i; j]) result
                      -> MkPrefix pref i i'
                      -> MkPrefix pref j j'
                      -> entails S I G i' 
@@ -178,21 +191,21 @@ type entails :: substrate => infostrate => varDecl => infon => P =
                      -> entails S I G result
 
   | Entails_And_Elim1 : S:substrate -> I:infostrate -> G:varDecl
-     -> i : infon -> i': infon
-     -> j : infon
-     -> pref : list infon 
-     -> hyp : infon
-     -> MkPrefix pref (And i j) hyp
+     -> i : term -> i': term
+     -> j : term
+     -> pref : list term 
+     -> hyp : term
+     -> MkPrefix pref (App AndInfon [i; j]) hyp
      -> MkPrefix pref i i'
      -> entails S I G hyp
      -> entails S I G i'
 	 
   | Entails_W_Imp_Intro : S:substrate -> I:infostrate -> G:varDecl 
-                      -> i:infon
-                      -> j:infon -> j':infon 
-                      -> result:infon
-                      -> pref: list infon
-                      -> MkPrefix pref (Implies i j) result
+                      -> i:term
+                      -> j:term -> j':term 
+                      -> result:term
+                      -> pref: list term
+                      -> MkPrefix pref (App ImpliesInfon [i; j]) result
                       -> MkPrefix pref j j'
                       -> entails S I G j' 
                       -> entails S I G result
@@ -202,13 +215,13 @@ type entails :: substrate => infostrate => varDecl => infon => P =
 type Typing :: varDecl => term => typ => P =
    | Typing_var : g:varDecl -> x:var -> t:typ -> Mem (x,t) g -> Typing g (VarTerm x) t
 *)
-(* val subst: i:infon -> x:var -> u:term -> (i':infon * Subst i x u i') *)
+(* val subst: i:term -> x:var -> u:term -> (i':term * Subst i x u i') *)
 (* let subst i x u = raise "todo" *)
 
-type Subst :: infon => var => term => infon => P = 
-   | Subst_admit : i:infon -> x:var -> t:term -> i':infon -> Subst i x t i'
+type Subst :: term => var => term => term => P = 
+   | Subst_admit : i:term -> x:var -> t:term -> i':term -> Subst i x t i'
 
-val subst: i:infon -> x:var -> u:term -> (i':infon * Subst i x u i')
+val subst: i:term -> x:var -> u:term -> (i':term * Subst i x u i')
 let subst i x u = raise "todo"
 
 (************************)
@@ -216,12 +229,12 @@ let subst i x u = raise "todo"
 (************************) 
 
 val doDerive: S:substrate -> I:infostrate -> G:varDecl 
-           -> pref:prefix -> i:infon 
-           -> option (i':infon * MkPrefix pref i i' * entails S I G i')
+           -> pref:prefix -> i:term 
+           -> option (i':term * MkPrefix pref i i' * entails S I G i')
 let rec doDerive _S _I _G pref inf = 
   let memInfostrate_inf = memInfostrate inf _I in
   match inf with 
-  | Empty -> let (j, m) = mkPrefix pref inf in
+  | App(EmptyInfon, [])-> let (j, m) = mkPrefix pref inf in
 		              (* if unable to make F* prove sth, put in a runtime check *)
 			          (* if j = Empty then *)
                    Some((j, m, 
@@ -234,7 +247,7 @@ let rec doDerive _S _I _G pref inf =
 	     | None -> raise "assert false"
          | Some mis -> Some((j, m, Entails_Hyp_Knowledge _S _I _G i mis)))
 		 
-  | AsInfon q -> 
+  | App(AsInfon, [SubstrateQueryTerm q]) -> 
       (match pref with
          | [] -> let (j, m) = mkPrefix pref inf in
              (match memSubstrate q _S with 
@@ -249,7 +262,7 @@ let rec doDerive _S _I _G pref inf =
              let (j, m) = mkPrefix pref inf in
 	         Some((j, m, Entails_Q_Intro _S _I _G x i i' j pref (*m*) mi ei)))
 	 
-  | And i j ->
+  | App(AndInfon, [i; j]) -> (* TODO: extend to n variables *)
       (match (doDerive _S _I _G pref i, doDerive _S _I _G pref j) with
 	     | (None, _) -> None
 	     | (_, None) -> None
@@ -258,7 +271,7 @@ let rec doDerive _S _I _G pref inf =
 		      Some((a, m,
                     Entails_And_Intro _S _I _G i i' j j' a pref m mi mj ei ej)))
 					
-  | Implies i j ->
+  | App(ImpliesInfon, [i; j]) ->
       (match doDerive _S _I _G pref j with
 	     | None -> None
          | Some((j', mj, ej)) ->
